factored out a separate lemma to prove

src/tls/TLS.fst
@@ -145,6 +145,14 @@ opaque type trigger2 (x:nat) (y:nat) = True
    
    Later, we generalize over k, using the ghost_lemma combinator to introduce the quantifier.
 *) 
+open FStar.Set
+
+assume val equal_on_disjoint: s1:set rid -> s2:set rid{disjoint_regions s1 s2} -> r:rid{mem r s1} -> h0:t -> h1:t{modifies (Set.singleton r) h0 h1} -> Lemma (equal_on s2 h0 h1)
+// let equal_on_disjoint s1 s2 r h0 h1 = cut (modifies s1 h0 h1)
+
+val disjoint_regions_sym: s1:set rid -> s2:set rid{disjoint_regions s1 s2} -> Lemma (disjoint_regions s2 s1)
+let disjoint_regions_sym s1 s2 = ()
+
 val frame_epoch_k: c:connection ->  j:nat -> h0:HyperHeap.t -> h1:HyperHeap.t -> k:nat -> Ghost unit 
   (requires
     epochs_inv c h0 /\
@@ -167,16 +175,14 @@ let frame_epoch_k c j h0 h1 k =
   let e_k = Seq.index es k in
   let wr_j = writer_epoch e_j in
   if k<>j
-  then (assert (disjoint_regions (regions e_j) (regions e_k));
-//        assume (forall r. Set.mem r (regions e_k) ==> Map.contains h0 r);
-        assume (equal_on (regions e_k) h0 h1); //TODO!
+  then (equal_on_disjoint (regions e_j) (regions e_k) (region wr_j) h0 h1;
         frame_st_enc_inv (writer_epoch e_k) h0 h1;
         frame_decrypt (reader_epoch e_k) h0 h1;
         ())
   else (let r_k = reader_epoch e_k in
-        assert (epoch_region_inv r_k wr_j);
-        assert (disjoint_regions (regions_of (reader_epoch e_k)) (regions_of wr_j));
-        assume (equal_on (regions_of r_k) h0 h1); //TODO!
+        // assert (epoch_region_inv r_k wr_j);
+        disjoint_regions_sym (regions_of (reader_epoch e_k)) (regions_of wr_j);
+	equal_on_disjoint (regions_of wr_j) (regions_of (reader_epoch e_k)) (region wr_j) h0 h1;
         frame_decrypt (reader_epoch e_k) h0 h1)
  
 val frame_epoch: c:connection ->  j:nat -> h0:HyperHeap.t -> h1:HyperHeap.t -> Lemma 
